theories/Coherence/AddParams.v
@@ -1,0 +1,37 @@
+Require Import Util CSet IL Annotation MapDefined.
+Require Import Sim.
+Require Import Invariance Delocation DelocationAlgo DelocationCorrect.
+Require Import Liveness LabelsDefined.
+
+Arguments sim S {H} S' {H0} r t _ _.
+
+Definition addParams (s:IL.stmt) (lv:ann (set var)) : IL.stmt :=
+  let additional_params := fst (computeParameters nil nil nil s lv) in
+  compile nil s additional_params.
+
+Lemma addParams_correct (E:onv val) (ili:IL.stmt) lv
+  : defined_on (getAnn lv) E
+    -> live_sound Liveness.Imperative nil nil ili lv
+    -> noUnreachableCode LabelsDefined.isCalled ili
+    -> sim I.state F.state bot3 Sim
+          (nil, E, ili)
+          (nil:list F.block, E, addParams ili lv).
+Proof with eauto.
+  intros. subst. unfold addParams.
+  eapply sim_trans with (S2:=I.state).
+  - eapply bisim_sim.
+    eapply correct; eauto.
+    + eapply is_trs; eauto...
+    + eapply (@live_sound_compile nil)...
+      eapply is_trs...
+      eapply is_live...
+  - eapply bisim_sim.
+    eapply bisim_sym.
+    eapply (@srdSim_sim nil nil nil nil nil);
+      [ | isabsurd | econstructor | reflexivity | | econstructor ].
+    + eapply trs_srd; eauto.
+      eapply is_trs...
+    + eapply (@live_sound_compile nil nil nil)...
+      eapply is_trs...
+      eapply is_live...
+Qed.
